reln.sml
@@ -1,0 +1,35 @@
+(*
+To define a rel by recursion.
+P(a0,b0) <=> R(a0,b0) & 
+(!a b. P(a,b) ==> !a' b'. Q(a,b,a',b') ==> 
+ P(a',b'))
+
+!a b. P(a,b) <=>
+ !ss. (R(a0,b0) <=> IN(Pair(a0,b0),ss)) &
+      !a1 b1. IN(Pair(a1,b1),ss) ==>
+      !a1' b1'. Q(a1,b1,a1',b1') ==> 
+      IN(Pair(a1',b1'),ss)
+
+
+P_ind
+ind principle:
+((R(a0,b0) ==> P1(a0,b0)) &
+!a b. P1(a,b) ==> 
+  !a' b'. Q(a,b,a',b') ==> P1(a',b')) ==>
+!a b. P(a,b) ==> P1(a,b)
+
+P_rules:
+
+(R(a0,b0) ==> P(a0,b0)) & 
+!a b. P(a,b) ==> 
+ !a' b'.Q(a,b,a',b') ==> P(a',b')
+
+
+P_cases:
+
+!a b. P(a,b) <=> 
+ (R(a,b)) |
+ ?a0 b0. Q(a0,b0,a,b) & P(a0,b0)
+
+
+*)
