SEARList.sml
@@ -1195,7 +1195,19 @@ val _ = new_fun "App" (mem_sort (mk_set "B"),
 val rel2fun = store_ax("rel2fun",
 “!A B R:A->B. isFun(R) ==> ?!f:A~>B. !a b. App(f,a) = b <=> Holds(R,a,b)”)
 
+val asF_def = rel2fun |> spec_all |> undisch
+                      |> uex_expand |> ex2fsym0 "asF" ["R"]
+                      |> disch_all |> gen_all
+                      |> store_as "asF_def";
 
+val asF_App = asF_def |> spec_all |> undisch |> conjE1
+                      |> disch_all |> gen_all
+                      |> store_as "asF_App";
+
+val is_asF = asF_def |> spec_all |> undisch |> conjE2
+                      |> disch_all |> gen_all
+                      |> store_as "is_asF";
+ 
 local
 val l = fVar_Inst 
 [("P",([("a",mem_sort (mk_set "A")),("b",mem_sort (mk_set "B"))],
@@ -1233,19 +1245,41 @@ val _ = new_fun "o1" (fun_sort (mk_set "A") (mk_set "C"),
                      [("phi",fun_sort (mk_set "B") (mk_set "C")),
                       ("psi",fun_sort (mk_set "A") (mk_set "B"))])
 
-
+local
+val l = fVar_Inst 
+[("P",([("a",mem_sort (mk_set "A")),("b",mem_sort (mk_set "B"))],
+ “App(f:A~>B,a) = b”))] 
+(AX1 |> qspecl [‘A’, ‘B’] |> uex_expand)
+in
 val asR_ex = prove_store("asR_ex",
 e0
-(cheat)
+(rpt strip_tac >> strip_assume_tac l >>
+ qexists_tac ‘R’ >> arw[])
 (form_goal
  “!A B f:A~>B.?R.!a b. Holds(R,a,b) <=> App(f,a) = b”));
+end
 
 val asR_def = asR_ex |> spec_all |> ex2fsym0 "asR" ["f"]
                      |> gen_all
 
+val asR_Fun = prove_store("asR_Fun",
+e0
+(rpt strip_tac >> rw[Fun_expand] >>
+ rw[asR_def] >> rpt strip_tac (* 2 *)
+ >-- (qexists_tac ‘App(f,a)’ >> rw[]) >>
+ pop_assum (assume_tac o GSYM) >> arw[])
+(form_goal
+ “!A B f:A~>B. isFun(asR(f))”));
+
 val o1_ex = prove_store("o1_ex",
 e0
-(cheat)
+(rpt strip_tac >>
+ qexists_tac ‘asF(asR(psi) o asR(phi))’ >> 
+ qsspecl_then [‘psi’] assume_tac asR_Fun >>
+ qsspecl_then [‘phi’] assume_tac asR_Fun >>
+ qby_tac ‘isFun(asR(psi) o asR(phi))’ 
+ >-- (irule o_Fun >> arw[]) >>
+ drule asF_App >> arw[])
 (form_goal
  “!A B phi:A~>B C psi:B~>C. ?f:A~>C. 
  !a c. App(f,a) = c <=> Holds(asR(psi) o asR(phi),a,c)”));
@@ -1261,5 +1295,446 @@ e0
 (form_goal
  “!A B f:A~>B C g:B~>C a. App(g,(App(f,a))) = App(o1(g,f),a)”));
 
+
+(*Thm_2_3_5*)
+val To1_fun_uex = prove_store("To1_fun_uex",
+e0
+(strip_tac >> uex_tac >> qexists_tac ‘asF(To1(A))’ >> rw[] >>
+ strip_tac >> irule is_asF >> rw[To1_Fun] >> rw[dot_def] >>
+ rpt strip_tac >> 
+ qspecl_then [‘A’] assume_tac To1_Fun >>
+ drule Eval_def >> arw[dot_def]
+ )
+(form_goal
+ “!A. ?!f:A~>1. T”));
+
+val _ = new_pred "isPr" 
+                 [("pi1",fun_sort (Cross (mk_set "A") (mk_set "B")) (mk_set "A")),("pi2",fun_sort (Cross (mk_set "A") (mk_set "B")) (mk_set "B"))]
+
+val isPr_def = store_ax("isPr_def",
+“!A B pj1:A * B ~>A pj2: A * B ~>B. isPr(pj1,pj2) <=>
+ !X f:X~>A g:X~>B.?!fg:X ~> A * B. o1(pj1,fg) = f &  o1(pj2,fg) = g”)
+
+val pi1_ex = prove_store("pi1_ex",
+e0
+(rpt strip_tac >> qexists_tac ‘asF(p1(A,B))’ >> rw[])
+(form_goal “!A B. ?pi1. asF(p1(A,B)) = pi1”));
+
+val pi1_def = pi1_ex |> spec_all |> ex2fsym0 "pi1" ["A","B"]
+                     |> gen_all |> store_as "pi1_def";
+
+val pi2_ex = prove_store("pi2_ex",
+e0
+(rpt strip_tac >> qexists_tac ‘asF(p2(A,B))’ >> rw[])
+(form_goal “!A B. ?pi2. asF(p2(A,B)) = pi2”));
+
+
+val pi2_def = pi2_ex |> spec_all |> ex2fsym0 "pi2" ["A","B"]
+                     |> gen_all |> store_as "pi2_def";
+
+val asR_o = prove_store("o_asR",
+e0
+(rpt strip_tac >> irule $ iffRL R_EXT >> rpt strip_tac >>
+ rw[asR_def] >> rw[o1_def])
+(form_goal
+ “!A B f:A~>B C g:B~> C. asR(g) o asR(f) = asR(o1(g,f))”));
+
+
+val asF_o1 = prove_store("asF_o1",
+e0
+(rpt strip_tac >> irule fun_ext0 >> strip_tac >>
+ rw[o1_def] >>
+ drule asR_asF >> rev_drule asR_asF >> arw[] >>
+ qby_tac ‘isFun(g o f)’ >-- (irule o_Fun >> arw[]) >>
+ drule Eval_def >> arw[] >> drule asF_App >> arw[])
+(form_goal
+ “!A B f:A->B C g:B-> C. 
+  isFun(f) & isFun(g) ==>
+  o1(asF(g),asF(f)) = asF(g o f)”));
+
+
+val Eval_asR = prove_store("Eval_asR",
+e0
+(rpt strip_tac >> flip_tac >> rw[GSYM asR_def] >>
+ qsspecl_then [‘f’] assume_tac asR_Fun >>
+ drule Holds_Eval >> arw[])
+(form_goal
+ “!A B f:A~>B a. Eval(asR(f),a) = App(f,a)”));
+
+val asF_asR = prove_store("asF_asR",
+e0
+(rpt strip_tac >> irule fun_ext0 >> 
+ qsspecl_then [‘f’] assume_tac asR_Fun >>
+ strip_tac >> drule asF_App >> arw[] >>
+ rw[asR_def])
+(form_goal
+ “!A B f:A~>B. asF(asR(f)) =f”));
+
+val asR_asF = prove_store("asR_asF",
+e0
+(rpt strip_tac >> irule $ iffRL R_EXT >>
+ rw[asR_def] >> drule asF_App >> arw[])
+(form_goal
+ “!A B f:A->B. isFun(f) ==> asR(asF(f)) =f”));
+
+val asR_eq_eq = prove_store("asR_eq_eq",
+e0
+(rpt strip_tac >> dimp_tac >> strip_tac >> arw[] >>
+ once_rw[GSYM asF_asR] >> arw[])
+(form_goal
+ “!A B f:A~>B g. asR(f) = asR(g) <=> f = g”));
+
+
+val Pf_ex = prove_store("Pf_ex",
+e0
+(rpt strip_tac >> rw[isPr_def] >> rpt strip_tac >>
+ uex_tac >> qexists_tac ‘asF(Pa(asR(f),asR(g)))’ >>
+ qsspecl_then [‘f’] assume_tac asR_Fun >>
+ qsspecl_then [‘g’] assume_tac asR_Fun >>
+ qspecl_then [‘A’,‘B’] assume_tac p12_Fun >>
+ qby_tac ‘isFun(Pa(asR(f),asR(g)))’
+ >-- (irule Pa_Fun >> arw[]) >> 
+ qby_tac
+ ‘o1(pi1(A, B), asF(Pa(asR(f), asR(g)))) = f’
+ >-- (rw[GSYM pi1_def] >> 
+     qsspecl_then [‘Pa(asR(f),asR(g))’,‘p1(A,B)’] assume_tac 
+     asF_o1 >> rfs[] >>
+     qsspecl_then [‘asR(f)’,‘asR(g)’] assume_tac p1_of_Pa >>
+     rfs[] >> rw[asF_asR]) >>
+ arw[] >> 
+ qby_tac
+ ‘o1(pi2(A, B), asF(Pa(asR(f), asR(g)))) = g’
+ >-- (rw[GSYM pi2_def] >> 
+     qsspecl_then [‘Pa(asR(f),asR(g))’,‘p2(A,B)’] assume_tac 
+     asF_o1 >> rfs[] >>
+     qsspecl_then [‘asR(f)’,‘asR(g)’] assume_tac p2_of_Pa >>
+     rfs[] >> rw[asF_asR]) >>
+ arw[] >> rpt strip_tac >>
+ irule $ iffLR asR_eq_eq >>
+ qby_tac ‘asR(asF(Pa(asR(f), asR(g)))) = Pa(asR(f), asR(g))’ 
+ >-- (irule asR_asF >> arw[]) >>
+ arw[] >> irule is_Pa >> arw[] >>
+ rw[asR_Fun] >> 
+ qsuff_tac ‘p2(A, B) o asR(fg')  = asR(o1(pi2(A, B), fg')) &
+            p1(A, B) o asR(fg')  = asR(o1(pi1(A, B), fg'))’
+ >-- (strip_tac >> arw[]) >>
+ arw[] >> fs[GSYM pi1_def,GSYM pi2_def] >>
+ qsspecl_then [‘fg'’] assume_tac asR_Fun >>
+ qsspecl_then [‘asR(fg')’,‘p1(A, B)’] assume_tac asF_o1 >>
+ rfs[] >>
+ qsspecl_then [‘asR(fg')’,‘p2(A, B)’] assume_tac asF_o1 >>
+ rfs[] >>
+ fs[asF_asR] >> 
+ qpick_x_assum
+ ‘asF(p1(A, B) o asR(fg')) = f’ (assume_tac o GSYM) >> arw[] >>
+ qpick_x_assum 
+ ‘asF(p2(A, B) o asR(fg')) = g’ (assume_tac o GSYM) >> arw[] >>
+ strip_tac >> 
+ irule $ GSYM asR_asF >> irule o_Fun >> arw[])
+(form_goal “!A B. isPr(pi1(A,B),pi2(A,B))”));
+ 
+val Pf_def = Pf_ex |> rewr_rule[isPr_def]
+                   |> spec_all
+                   |> uex_expand |> ex2fsym0 "Pf" ["f","g"] 
+                   |> gen_all
+
+val pi1_of_Pair = prove_store("pi1_of_Pair",
+e0
+(rpt strip_tac >> rw[GSYM pi1_def] >> qspecl_then [‘A’,‘B’] assume_tac p1_Fun >> drule App_asF_Eval >> arw[] >> rw[Eval_p1_Pair])
+(form_goal
+ “!A B a b. App(pi1(A,B),Pair(a,b)) = a”));
+
+val pi2_of_Pair = prove_store("pi2_of_Pair",
+e0
+(rpt strip_tac >> rw[GSYM pi2_def] >> qspecl_then [‘A’,‘B’] assume_tac p2_Fun >> drule App_asF_Eval >> arw[] >> rw[Eval_p2_Pair])
+(form_goal
+ “!A B a b. App(pi2(A,B),Pair(a,b)) = b”));
+
+val List_rec_mem = prove_store("List_rec_mem",
+e0
+(rpt strip_tac >> drule List_rec >>
+ pop_assum (strip_assume_tac o uex_expand) >>
+ uex_tac >> qexists_tac ‘f’ >> arw[] >> rpt strip_tac (* 2 *)
+ >-- (rw[GSYM CONS_def] >>
+ irule $ iffLR Eval_o_l >> arw[] >> rw[Cons_def] >>
+ irule $ iffRL Eval_o_l >> arw[] >>
+ qby_tac ‘isFun(p1(A,List(A))) & isFun(f o p2(A,List(A)))’ 
+ >-- (rw[p1_Fun] >> irule o_Fun >> arw[p2_Fun]) >>
+ drule Pa_Fun >> arw[] >> irule Eval_input_eq >>
+ drule Eval_Pa_Pair >> arw[] >> rw[Eval_p1_Pair] >>
+ rw[Pair_eq_eq] >> irule $ iffRL Eval_o_l >>
+ arw[Eval_p2_Pair,p2_Fun]) >>
+ first_x_assum irule >> arw[] >> irule $ iffRL FUN_EXT >>
+ qby_tac ‘isFun(f' o Cons(A))’ >-- (irule o_Fun >> arw[Cons_def]) >>
+ qby_tac ‘isFun(t o Pa(p1(A, List(A)), f' o p2(A, List(A))))’ 
+ >-- (irule o_Fun >> arw[] >> irule Pa_Fun >> rw[p1_Fun] >>
+      irule o_Fun >> arw[p2_Fun]) >>
+ arw[] >> strip_tac >> irule $ iffRL Eval_o_l >>
+ arw[Cons_def] >> 
+ qsspecl_then [‘a’] 
+ (x_choosel_then ["a0","l0"] assume_tac) Pair_has_comp >>
+ arw[CONS_def] >> flip_tac >> irule $ iffRL Eval_o_l >>
+ arw[] >>
+ qby_tac ‘isFun(Pa(p1(A, List(A)), f' o p2(A, List(A))))’
+ >-- (irule Pa_Fun >> rw[p1_Fun] >> irule o_Fun >> arw[p2_Fun]) >>
+ arw[] >> irule Eval_input_eq >> 
+ qby_tac
+ ‘isFun(p1(A,List(A))) & isFun(f' o p2(A,List(A)))’
+ >-- (rw[p1_Fun] >> irule o_Fun >> arw[p2_Fun]) >>
+ drule Eval_Pa_Pair >> arw[Eval_p1_Pair] >> 
+ rw[Pair_eq_eq] >> irule $ iffRL Eval_o_l >> 
+ arw[p2_Fun] >> rw[Eval_p2_Pair])
+(form_goal
+ “!X x:mem(X) A t. isFun(t) ==> ?!f. isFun(f) & 
+  Eval(f,Nil(A)) = x &
+  !a l. Eval(f,CONS(a,l)) = Eval(t,Pair(a,Eval(f,l)))”));
+
+val App_asF_Eval = prove_store("App_asF_Eval",
+e0
+(rpt strip_tac >> drule asF_def >> arw[] >>
+ drule Holds_Eval >> arw[])
+(form_goal
+ “!A B f:A->B. isFun(f) ==> !a.App(asF(f), a) = Eval(f,a)”));
+
+
+val App_Eval_asR = prove_store("App_Eval_asR",
+e0
+(rpt strip_tac >> rw[GSYM asR_def] >> irule Holds_Eval >>
+ rw[asR_Fun])
+(form_goal
+ “!A B f:A~>B. !a.App(f, a) = Eval(asR(f),a)”));
+
+
+val List_rec_fun = prove_store("List_rec_fun",
+e0
+(rpt strip_tac >> 
+ qsspecl_then [‘x’,‘asR(t)’] assume_tac List_rec_mem >>
+ qsspecl_then [‘t’] assume_tac asR_Fun >>
+ first_x_assum drule >>
+ pop_assum (strip_assume_tac o uex_expand) >>
+ drule App_asF_Eval >> uex_tac >>
+ qexists_tac ‘asF(f)’ >>
+ arw[] >> rw[GSYM App_Eval_asR] >> rpt strip_tac >>
+ irule $ iffLR asR_eq_eq >> drule asR_asF >> arw[] >>
+ first_x_assum irule >> arw[asR_Fun,GSYM App_Eval_asR])
+(form_goal
+ “!X x A t. ?!f:List(A)~> X. 
+ App(f,Nil(A)) = x &
+ !a l. App(f,CONS(a,l)) = App(t,Pair(a,App(f,l)))
+ ”));
+
+val Eval_o_p2 = prove_store("Eval_o_p2",
+e0
+(rpt strip_tac >> irule $ iffRL Eval_o_l >>
+ arw[p2_Fun] >> rw[Eval_p2_Pair])
+(form_goal
+ “!X B f:B->X. isFun(f) ==> !A a b. Eval(f o p2(A,B),Pair(a,b)) = Eval(f,b)”));
+
+val Eval_o_p1 = prove_store("Eval_o_p1",
+e0
+(rpt strip_tac >> irule $ iffRL Eval_o_l >>
+ arw[p1_Fun] >> rw[Eval_p1_Pair])
+(form_goal
+ “!X A f:A->X. isFun(f) ==> !B a b. Eval(f o p1(A,B),Pair(a,b)) = Eval(f,a)”));
+
+
+val Thm1_mem = prove_store("Thm1_fun",
+e0
+(rpt gen_tac >> disch_tac >> drule Thm1 >> 
+ pop_assum strip_assume_tac >> uex_tac >>
+ qexists_tac ‘f’ >> 
+ first_assum (qspecl_then [‘f’] assume_tac) >> fs[] >>
+ strip_tac (* 2 *)
+ >-- (rpt strip_tac (* 2 *) >-- 
+     (qby_tac ‘ Eval(g, a) = Eval(g o p1(A, 1),Pair(a,dot))’ 
+     >-- (flip_tac >> irule $ iffRL Eval_o_l >> rw[Eval_p1_Pair] >>
+         arw[p1_Fun]) >>
+     arw[] >>
+     qpick_x_assum ‘f o Pa(p1(A, 1), El(O) o p2(A, 1)) = g o p1(A, 1)’
+     (assume_tac o GSYM) >> arw[] >>
+     flip_tac >> irule  $ iffRL Eval_o_l  >>
+     qby_tac
+     ‘isFun(Pa(p1(A, 1), El(O) o p2(A, 1)))’
+     >-- (irule Pa_Fun >> rw[p1_Fun] >> irule o_Fun >>
+          rw[p2_Fun,El_Fun]) >> arw[] >>
+     irule Eval_input_eq >> 
+     qby_tac ‘isFun(p1(A,1)) & isFun(El(O) o p2(A,1))’ 
+     >-- (rw[p1_Fun] >> irule o_Fun >> rw[p2_Fun,El_Fun]) >>
+     drule Eval_Pa_Pair >> arw[] >> rw[Pair_eq_eq,Eval_p1_Pair] >>
+     irule $ iffRL Eval_o_l >> rw[El_Fun,p2_Fun] >>
+     rw[El_def,dot_def]) >>
+     qby_tac
+     ‘Eval(f, Pair(a, Suc(n))) = Eval(f o Pa(p1(A, N), SUC o p2(A, N)),Pair(a,n))’
+     >-- (flip_tac >> irule $ iffRL Eval_o_l >> 
+         qby_tac ‘isFun(p1(A,N)) & isFun(SUC o p2(A, N))’
+         >-- (rw[p1_Fun] >> irule o_Fun >> rw[SUC_Fun,p2_Fun]) >>
+         drule Pa_Fun >> arw[] >>
+         irule Eval_input_eq >> drule Eval_Pa_Pair >> 
+         arw[Eval_p1_Pair] >> rw[Pair_eq_eq] >> 
+         irule  $ iffRL Eval_o_l >> rw[p2_Fun,SUC_Fun] >>
+         rw[Suc_def,Eval_p2_Pair]) >>
+     arw[] >> pop_assum (K all_tac) >>
+     pop_assum (assume_tac o GSYM) >> arw[] >>
+     irule  $ iffRL Eval_o_l >> arw[] >>
+     qby_tac ‘isFun(Pa(id(A * N), f))’ 
+     >-- (irule Pa_Fun >> arw[id_Fun]) >>
+     arw[] >> irule Eval_input_eq >> 
+     qby_tac ‘isFun(id(A * N)) & isFun(f)’ 
+     >-- arw[id_Fun] >>
+     drule Eval_Pa_Pair >> arw[Eval_id]) >>
+rpt strip_tac >>  first_x_assum (irule o iffLR) >>
+arw[] >> strip_tac (* 2 *) >-- 
+(irule $ iffRL FUN_EXT >> rpt strip_tac (* 3 *)
+>-- (qsspecl_then [‘a’] (x_choosel_then ["a0","n0"] assume_tac)
+    Pair_has_comp >> arw[] >> irule $ iffRL Eval_o_l >>
+    arw[] >> 
+    qsspecl_then [‘id(A * N)’,‘f'’] assume_tac Pa_Fun >>
+    rfs[id_Fun] >> 
+    qsspecl_then [‘id(A * N)’,‘f'’] assume_tac Eval_Pa_Pair >>
+    rfs[id_Fun] >> rw[Eval_id] >> flip_tac >>
+    irule  $ iffRL Eval_o_l >> 
+    qby_tac ‘isFun(p1(A,N)) & isFun(SUC o p2(A,N))’
+    >-- (rw[p1_Fun] >> irule o_Fun >> rw[SUC_Fun,p2_Fun]) >>
+    arw[] >> drule Pa_Fun >> arw[] >> 
+    drule Eval_Pa_Pair >> arw[Eval_p1_Pair] >>
+    assume_tac SUC_Fun >> drule Eval_o_p2 >> arw[Suc_def])
+>-- (irule o_Fun >> arw[] >> irule Pa_Fun >> arw[id_Fun]) >>
+irule o_Fun >> arw[] >> irule Pa_Fun >> rw[p1_Fun] >>
+irule o_Fun >> rw[SUC_Fun,p2_Fun]) >>
+irule $ iffRL FUN_EXT  >> rpt strip_tac (* 3 *)
+>-- (qsspecl_then [‘a’] (x_choosel_then ["a0","n0"] assume_tac)
+    Pair_has_comp >> arw[] >>  irule $ iffRL Eval_o_l >> arw[] >>
+    qby_tac ‘isFun(p1(A,1)) & isFun(El(O) o p2(A, 1))’
+    >-- (rw[p1_Fun] >> irule o_Fun >> rw[El_Fun,p2_Fun]) >>
+    drule Pa_Fun >> arw[] >> drule Eval_Pa_Pair >> arw[] >>
+    rw[Eval_p1_Pair] >> qsspecl_then [‘O’] assume_tac El_Fun >>
+    drule Eval_o_p2 >> arw[] >> rw[dot_def,El_def] >> arw[] >>
+    rev_drule Eval_o_p1 >> arw[]) 
+>-- (irule o_Fun >> arw[] >> irule Pa_Fun >> rw[p1_Fun] >>
+    irule o_Fun >> rw[El_Fun,p2_Fun]) >>
+irule o_Fun >> arw[p1_Fun])
+(form_goal
+ “!A B g:A->B h : (A * N) * B -> B. 
+ isFun(g) & isFun(h) ==> 
+ ?!f:A * N -> B. 
+ isFun(f) & 
+ (!a.Eval(f, Pair(a,O)) = Eval(g,a)) &
+ (!a n. Eval(f,Pair(a,Suc(n))) = Eval(h,Pair(Pair(a,n),Eval(f,Pair(a,n)))))”));
+
+
+val Thm1_fun = prove_store("Thm1_fun",
+e0
+(rpt strip_tac >> uex_tac >> 
+ qby_tac ‘isFun(asR(g)) & isFun(asR(h))’
+ >-- rw[asR_Fun] >>
+ drule Thm1_mem >>
+ pop_assum (strip_assume_tac o uex_expand) >>
+ qexists_tac ‘asF(f)’ >>
+ strip_tac (* 2 *)
+ >-- (rpt strip_tac (* 2 *)
+     >-- (drule App_asF_Eval >> arw[] >> rw[Eval_asR]) >>
+     drule App_asF_Eval >> arw[] >> rw[Eval_asR]) >>
+ rpt strip_tac >> irule $ iffLR asR_eq_eq >>
+ drule asR_asF >> arw[] >>
+ first_x_assum irule >> rw[asR_Fun] >>
+ arw[Eval_asR])
+(form_goal
+ “!A B g:A~>B h : (A * N) * B ~> B. 
+  ?!f.
+     (!a.App(f, Pair(a,O)) = App(g,a)) &
+     (!a n. App(f,Pair(a,Suc(n))) = App(h,Pair(Pair(a,n),App(f,Pair(a,n)))))”));
+
+val Hd_def0 = List_rec_fun |> qspecl [‘A’,‘Arb(A)’,‘A’,‘pi1(A,A)’]
+                           |> uex_expand |> ex2fsym0 "Hd" ["A"]
+                           |> gen_all |> store_as "Hd_def0";
+
+val HD_ex = prove_store("HD_ex",
+e0
+(rpt strip_tac >> qexists_tac ‘App(Hd(A),l)’ >> rw[])
+(form_goal
+ “!A l. ?h. App(Hd(A),l) = h”));
+
+val HD_def = HD_ex |> spec_all |> ex2fsym0 "HD" ["l"]
+                   |> gen_all |> store_as "HD_def";
+
+val HD = prove_store("HD",
+e0
+(rpt strip_tac >> rw[GSYM HD_def] >>
+ qspecl_then [‘A’] strip_assume_tac Hd_def0 >>
+ arw[] >> rw[pi1_of_Pair])
+(form_goal
+ “!A a:mem(A) l.HD(CONS(a,l)) = a”));
+
+
+val CONS_ne_Nil = prove_store("CONS_ne_Nil",
+e0
+(rpt strip_tac >> ccontra_tac >>
+ qby_tac ‘sof(CONS(h,t)) = sof(Nil(A))’ 
+ >-- arw[] >>
+ fs[sof_Nil] >> pop_assum mp_tac >>
+ rw[GSYM CONS_eqn] >> rw[Ins_NONEMPTY])
+(form_goal “!A h t. ~(CONS(h,t) = Nil(A))”));
+
+local
+val l = 
+fVar_Inst [("P",([("l",mem_sort (rastt "List(A)")),
+                  ("t",mem_sort (rastt "List(A)"))],
+“(l = Nil(A) & t = Nil(A)) | (?h t0. l = CONS(h,t0) & t = t0)”))]
+(AX1 |> qspecl [‘List(A)’,‘List(A)’]) |> uex_expand
+in
+val Tl_ex0 = prove_store("Tl_ex0",
+e0
+(strip_tac >> strip_assume_tac l >>
+ pop_assum (K all_tac) >> qexists_tac ‘R’ >> 
+ qby_tac ‘isFun(R)’ >--
+ (rw[Fun_expand] >> rpt strip_tac (* 2 *)
+  >-- (qsspecl_then [‘a’] strip_assume_tac CONS_or_Nil 
+      >-- (arw[] >> qexists_tac ‘Nil(A)’ >> rw[]) >>
+      arw[] >> qexists_tac ‘l0’ >> disj2_tac >> 
+      qexistsl_tac [‘a0’,‘l0’] >> arw[]) >>
+  qsspecl_then [‘a’] strip_assume_tac CONS_or_Nil >--
+  (fs[] >> rfs[GSYM CONS_ne_Nil]) >>
+  fs[] >> rfs[CONS_ne_Nil] >> fs[CONS_eq_eq]) >>
+ arw[] >> drule $ GSYM Eval_def >> flip_tac >> arw[] >>
+ rpt strip_tac >> rw[CONS_ne_Nil] >>
+ qexistsl_tac [‘a’,‘l’] >> rw[])
+(form_goal
+ “!A. ?tl. isFun(tl) & Eval(tl,Nil(A)) = Nil(A) & 
+ (!a l. Eval(tl,CONS(a,l)) = l)”));
+end
+
+val Tl_ex = prove_store("Tl_ex",
+e0
+(strip_tac >>
+ qspecl_then [‘A’] strip_assume_tac Tl_ex0 >>
+ qexists_tac ‘asF(tl)’ >> drule App_asF_Eval >>
+ arw[])
+(form_goal
+ “!A. ?tl. App(tl,Nil(A)) = Nil(A) & 
+ (!a l. App(tl,CONS(a,l)) = l)”));
+
+val Tl_def =  Tl_ex |> spec_all |> ex2fsym0 "Tl" ["A"]
+                   |> gen_all |> store_as "Tl_def";
+
+val TL_ex = prove_store("TL_ex",
+e0
+(rpt strip_tac >> qexists_tac ‘App(Tl(A),l)’ >> rw[])
+(form_goal
+ “!A l. ?h. App(Tl(A),l) = h”));
+
+val TL_def = TL_ex |> spec_all |> ex2fsym0 "TL" ["l"]
+                   |> gen_all |> store_as "TL_def";
+ 
+val Cons_Fun = Cons_def |> spec_all |> conjE1 |> gen_all
+                        |> store_as "Cons_Fun";
+
+
+
+val TL = prove_store("TL",
+e0
+(rpt strip_tac >> rw[GSYM TL_def] >>
+ qspecl_then [‘A’] strip_assume_tac Tl_def >> arw[])
+(form_goal
+ “!A. TL(Nil(A)) = Nil(A) & !a:mem(A) l.TL(CONS(a,l)) = l”));
 
 (*seems that need to edit the input of Pa to be fun instead of rel.*)
